_build/default/core.ml
@@ -1,0 +1,172 @@
+
+type nat =
+| O
+| S of nat
+
+(** val app : 'a1 list -> 'a1 list -> 'a1 list **)
+
+let rec app l m =
+  match l with
+  | [] -> m
+  | a :: l1 -> a :: (app l1 m)
+
+(** val map : ('a1 -> 'a2) -> 'a1 list -> 'a2 list **)
+
+let rec map f = function
+| [] -> []
+| a :: t -> (f a) :: (map f t)
+
+(** val eqb : char list -> char list -> bool **)
+
+let rec eqb s1 s2 =
+  match s1 with
+  | [] -> (match s2 with
+           | [] -> true
+           | _::_ -> false)
+  | c1::s1' ->
+    (match s2 with
+     | [] -> false
+     | c2::s2' -> if (=) c1 c2 then eqb s1' s2' else false)
+
+type ident = char list
+
+type aexpr =
+| Var of ident
+| Cst of int
+| Add of aexpr * aexpr
+| Sub of aexpr * aexpr
+
+type bexpr =
+| Bcst of bool
+| Ble of aexpr * aexpr
+| Beq of aexpr * aexpr
+| Bnot of bexpr
+| Band of bexpr * bexpr
+
+type prog =
+| Skip
+| Ite of bexpr * prog * prog
+| Seq of prog * prog
+| Asg of char list * aexpr
+| Err
+| Loop of bexpr * prog
+
+module Oracle =
+ struct
+  (** val next_is_error : prog -> bool **)
+
+  let rec next_is_error = function
+  | Seq (p0, _) -> next_is_error p0
+  | Err -> true
+  | _ -> false
+ end
+
+module Symb =
+ struct
+  type store = ident -> aexpr
+
+  type state = (bexpr * store) * prog
+
+  (** val id : store **)
+
+  let id x =
+    Var x
+
+  (** val init : prog -> state **)
+
+  let init p =
+    (((Bcst true), id), p)
+
+  (** val update : store -> ident -> aexpr -> store **)
+
+  let update s x e y =
+    if eqb y x then e else s y
+
+  (** val aeval : store -> aexpr -> aexpr **)
+
+  let rec aeval s e = match e with
+  | Var x -> s x
+  | Cst _ -> e
+  | Add (e1, e2) -> Add ((aeval s e1), (aeval s e2))
+  | Sub (e1, e2) -> Sub ((aeval s e1), (aeval s e2))
+
+  (** val beval : store -> bexpr -> bexpr **)
+
+  let rec beval s e = match e with
+  | Bcst _ -> e
+  | Ble (e1, e2) -> Ble ((aeval s e1), (aeval s e2))
+  | Beq (e1, e2) -> Beq ((aeval s e1), (aeval s e2))
+  | Bnot e0 -> Bnot (beval s e0)
+  | Band (e1, e2) -> Band ((beval s e1), (beval s e2))
+
+  (** val is_error : state -> bool **)
+
+  let is_error = function
+  | (_, prog0) -> Oracle.next_is_error prog0
+ end
+
+type 'a stream = 'a __stream Lazy.t
+and 'a __stream =
+| Snil
+| Scons of 'a * 'a stream
+
+type 'a result =
+| Timeout
+| Found of 'a
+| NotFound
+
+(** val search : nat -> ('a1 -> bool) -> 'a1 stream -> 'a1 result **)
+
+let rec search fuel p s =
+  match fuel with
+  | O -> (match Lazy.force
+          s with
+          | Snil -> NotFound
+          | Scons (_, _) -> Timeout)
+  | S fuel0 ->
+    (match Lazy.force
+     s with
+     | Snil -> NotFound
+     | Scons (x, s0) -> if p x then Found x else search fuel0 p s0)
+
+type skip_case =
+| Is_skip
+| Is_not_skip
+
+(** val skip_dec : prog -> skip_case **)
+
+let skip_dec = function
+| Skip -> Is_skip
+| _ -> Is_not_skip
+
+(** val expand : bexpr -> Symb.store -> prog -> Symb.state list **)
+
+let rec expand path env = function
+| Ite (b, p1, p2) ->
+  (((Band (path, (Symb.beval env b))), env), p1) :: ((((Band (path, (Bnot
+    (Symb.beval env b)))), env), p2) :: [])
+| Seq (p1, p2) ->
+  (match skip_dec p1 with
+   | Is_skip -> ((path, env), p2) :: []
+   | Is_not_skip ->
+     map (fun pat -> let (y, p) = pat in (y, (Seq (p, p2))))
+       (expand path env p1))
+| Asg (x, e) -> ((path, (Symb.update env x (Symb.aeval env e))), Skip) :: []
+| Loop (b, p) ->
+  (((Band (path, (Symb.beval env b))), env), (Seq (p, (Loop (b,
+    p))))) :: ((((Band (path, (Bnot (Symb.beval env b)))), env), Skip) :: [])
+| _ -> []
+
+(** val reachable : Symb.state list -> Symb.state stream **)
+
+let rec reachable = function
+| [] -> lazy Snil
+| s :: l0 ->
+  let (p0, p) = s in
+  let (path, senv) = p0 in
+  lazy (Scons (s, (reachable (app l0 (expand path senv p)))))
+
+(** val find_bugs : nat -> prog -> Symb.state result **)
+
+let find_bugs fuel p =
+  search fuel Symb.is_error (reachable ((Symb.init p) :: []))
