_build/default/minibug.ml
@@ -1,0 +1,4 @@
+open Parser
+
+let () =
+  print_endline "hello"
