core.ml
@@ -1,0 +1,246 @@
+
+(** val app : 'a1 list -> 'a1 list -> 'a1 list **)
+
+let rec app l m =
+  match l with
+  | [] -> m
+  | a :: l1 -> a :: (app l1 m)
+
+(** val map : ('a1 -> 'a2) -> 'a1 list -> 'a2 list **)
+
+let rec map f = function
+| [] -> []
+| a :: t -> (f a) :: (map f t)
+
+(** val eqb : char list -> char list -> bool **)
+
+let rec eqb s1 s2 =
+  match s1 with
+  | [] -> (match s2 with
+           | [] -> true
+           | _::_ -> false)
+  | c1::s1' -> (match s2 with
+                | [] -> false
+                | c2::s2' -> if (=) c1 c2 then eqb s1' s2' else false)
+
+type ident = char list
+
+type aexpr =
+| Var of ident
+| Cst of int
+| Add of aexpr * aexpr
+| Sub of aexpr * aexpr
+
+type bexpr =
+| Bcst of bool
+| Ble of aexpr * aexpr
+| Beq of aexpr * aexpr
+| Bnot of bexpr
+| Band of bexpr * bexpr
+
+type prog =
+| Skip
+| Ite of bexpr * prog * prog
+| Seq of prog * prog
+| Asg of char list * aexpr
+| Err
+| Loop of bexpr * prog
+
+module Oracle =
+ struct
+  (** val next_is_error : prog -> bool **)
+
+  let rec next_is_error = function
+  | Seq (p0, _) -> next_is_error p0
+  | Err -> true
+  | _ -> false
+ end
+
+module Symb =
+ struct
+  type store = ident -> aexpr
+
+  type state = (bexpr * store) * prog
+
+  (** val id : store **)
+
+  let id x =
+    Var x
+
+  (** val init : prog -> state **)
+
+  let init p =
+    (((Bcst true), id), p)
+
+  (** val path : state -> bexpr **)
+
+  let path = function
+  | (p, _) -> let (path0, _) = p in path0
+
+  (** val update : store -> ident -> aexpr -> store **)
+
+  let update s x e y =
+    if eqb y x then e else s y
+
+  (** val aeval : store -> aexpr -> aexpr **)
+
+  let rec aeval s e = match e with
+  | Var x -> s x
+  | Cst _ -> e
+  | Add (e1, e2) -> Add ((aeval s e1), (aeval s e2))
+  | Sub (e1, e2) -> Sub ((aeval s e1), (aeval s e2))
+
+  (** val beval : store -> bexpr -> bexpr **)
+
+  let rec beval s e = match e with
+  | Bcst _ -> e
+  | Ble (e1, e2) -> Ble ((aeval s e1), (aeval s e2))
+  | Beq (e1, e2) -> Beq ((aeval s e1), (aeval s e2))
+  | Bnot e0 -> Bnot (beval s e0)
+  | Band (e1, e2) -> Band ((beval s e1), (beval s e2))
+
+  (** val is_error : state -> bool **)
+
+  let is_error = function
+  | (_, prog0) -> Oracle.next_is_error prog0
+ end
+
+type 'a stream = 'a __stream Lazy.t
+and 'a __stream =
+| Snil
+| Scons of 'a * 'a stream
+
+type 'a result =
+| Timeout
+| Found of 'a
+| NotFound
+
+(** val search_opt : int -> ('a1 -> 'a2 option) -> 'a1 stream -> 'a2 result **)
+
+let rec search_opt fuel p s =
+  (fun fO fS n -> if n=0 then fO () else fS (n-1))
+    (fun _ -> match Lazy.force
+              s with
+              | Snil -> NotFound
+              | Scons (_, _) -> Timeout)
+    (fun fuel0 ->
+    match Lazy.force
+    s with
+    | Snil -> NotFound
+    | Scons (x, s0) -> (match p x with
+                        | Some x0 -> Found x0
+                        | None -> search_opt fuel0 p s0))
+    fuel
+
+(** val search : int -> ('a1 -> bool) -> 'a1 stream -> 'a1 result **)
+
+let rec search fuel p s =
+  (fun fO fS n -> if n=0 then fO () else fS (n-1))
+    (fun _ -> match Lazy.force
+              s with
+              | Snil -> NotFound
+              | Scons (_, _) -> Timeout)
+    (fun fuel0 ->
+    match Lazy.force
+    s with
+    | Snil -> NotFound
+    | Scons (x, s0) -> if p x then Found x else search fuel0 p s0)
+    fuel
+
+type skip_case =
+| Is_skip
+| Is_not_skip
+
+(** val skip_dec : prog -> skip_case **)
+
+let skip_dec = function
+| Skip -> Is_skip
+| _ -> Is_not_skip
+
+(** val expand : bexpr -> Symb.store -> prog -> Symb.state list **)
+
+let rec expand path0 env = function
+| Ite (b, p1, p2) ->
+  (((Band (path0, (Symb.beval env b))), env), p1) :: ((((Band (path0, (Bnot
+    (Symb.beval env b)))), env), p2) :: [])
+| Seq (p1, p2) ->
+  (match skip_dec p1 with
+   | Is_skip -> ((path0, env), p2) :: []
+   | Is_not_skip ->
+     map (fun pat -> let (y, p) = pat in (y, (Seq (p, p2)))) (expand path0 env p1))
+| Asg (x, e) -> ((path0, (Symb.update env x (Symb.aeval env e))), Skip) :: []
+| Loop (b, p) ->
+  (((Band (path0, (Symb.beval env b))), env), (Seq (p, (Loop (b, p))))) :: ((((Band (path0,
+    (Bnot (Symb.beval env b)))), env), Skip) :: [])
+| _ -> []
+
+(** val reachable : Symb.state list -> Symb.state stream **)
+
+let rec reachable = function
+| [] -> lazy Snil
+| s :: l0 ->
+  let (p0, p) = s in
+  let (path0, senv) = p0 in lazy (Scons (s, (reachable (app l0 (expand path0 senv p)))))
+
+module NaiveBugFinder =
+ struct
+  module Spec =
+   struct
+   end
+
+  (** val find_bugs : int -> prog -> Symb.state result **)
+
+  let find_bugs fuel p =
+    search fuel Symb.is_error (reachable ((Symb.init p) :: []))
+ end
+
+type partial_store = (ident * int) list
+
+type solver_result =
+| SAT of partial_store
+| UNSAT
+| TIMEOUT
+
+module type SOLVER =
+ sig
+  val check_sat : bexpr -> solver_result
+ end
+
+module BugFinder =
+ functor (Solver:SOLVER) ->
+ struct
+  module Spec =
+   struct
+   end
+
+  type bug =
+  | SureBug of partial_store
+  | UnsureBug of bexpr
+
+  (** val bug_rect : (partial_store -> 'a1) -> (bexpr -> 'a1) -> bug -> 'a1 **)
+
+  let bug_rect f f0 = function
+  | SureBug wit -> f wit
+  | UnsureBug path0 -> f0 path0
+
+  (** val bug_rec : (partial_store -> 'a1) -> (bexpr -> 'a1) -> bug -> 'a1 **)
+
+  let bug_rec f f0 = function
+  | SureBug wit -> f wit
+  | UnsureBug path0 -> f0 path0
+
+  (** val is_error : Symb.state -> bug option **)
+
+  let is_error s =
+    if Symb.is_error s
+    then (match Solver.check_sat (Symb.path s) with
+          | SAT sol -> Some (SureBug sol)
+          | UNSAT -> None
+          | TIMEOUT -> Some (UnsureBug (Symb.path s)))
+    else None
+
+  (** val find_bugs : int -> prog -> bexpr -> bug result **)
+
+  let find_bugs fuel p ass =
+    search_opt fuel is_error (reachable (((ass, (fun x -> Var x)), p) :: []))
+ end
