core.mli
@@ -1,0 +1,120 @@
+
+val app : 'a1 list -> 'a1 list -> 'a1 list
+
+val map : ('a1 -> 'a2) -> 'a1 list -> 'a2 list
+
+val eqb : char list -> char list -> bool
+
+type ident = char list
+
+type aexpr =
+| Var of ident
+| Cst of int
+| Add of aexpr * aexpr
+| Sub of aexpr * aexpr
+
+type bexpr =
+| Bcst of bool
+| Ble of aexpr * aexpr
+| Beq of aexpr * aexpr
+| Bnot of bexpr
+| Band of bexpr * bexpr
+
+type prog =
+| Skip
+| Ite of bexpr * prog * prog
+| Seq of prog * prog
+| Asg of char list * aexpr
+| Err
+| Loop of bexpr * prog
+
+module Oracle :
+ sig
+  val next_is_error : prog -> bool
+ end
+
+module Symb :
+ sig
+  type store = ident -> aexpr
+
+  type state = (bexpr * store) * prog
+
+  val id : store
+
+  val init : prog -> state
+
+  val path : state -> bexpr
+
+  val update : store -> ident -> aexpr -> store
+
+  val aeval : store -> aexpr -> aexpr
+
+  val beval : store -> bexpr -> bexpr
+
+  val is_error : state -> bool
+ end
+
+type 'a stream = 'a __stream Lazy.t
+and 'a __stream =
+| Snil
+| Scons of 'a * 'a stream
+
+type 'a result =
+| Timeout
+| Found of 'a
+| NotFound
+
+val search_opt : int -> ('a1 -> 'a2 option) -> 'a1 stream -> 'a2 result
+
+val search : int -> ('a1 -> bool) -> 'a1 stream -> 'a1 result
+
+type skip_case =
+| Is_skip
+| Is_not_skip
+
+val skip_dec : prog -> skip_case
+
+val expand : bexpr -> Symb.store -> prog -> Symb.state list
+
+val reachable : Symb.state list -> Symb.state stream
+
+module NaiveBugFinder :
+ sig
+  module Spec :
+   sig
+   end
+
+  val find_bugs : int -> prog -> Symb.state result
+ end
+
+type partial_store = (ident * int) list
+
+type solver_result =
+| SAT of partial_store
+| UNSAT
+| TIMEOUT
+
+module type SOLVER =
+ sig
+  val check_sat : bexpr -> solver_result
+ end
+
+module BugFinder :
+ functor (Solver:SOLVER) ->
+ sig
+  module Spec :
+   sig
+   end
+
+  type bug =
+  | SureBug of partial_store
+  | UnsureBug of bexpr
+
+  val bug_rect : (partial_store -> 'a1) -> (bexpr -> 'a1) -> bug -> 'a1
+
+  val bug_rec : (partial_store -> 'a1) -> (bexpr -> 'a1) -> bug -> 'a1
+
+  val is_error : Symb.state -> bug option
+
+  val find_bugs : int -> prog -> bexpr -> bug result
+ end
