_build/default/README.md
@@ -1,0 +1,5 @@
+# minibug
+
+Concise and documented Coq formalization of a symbolic bug finder for IMP
+
+
